new theorems and properties

Lambda/Defs.lean
@@ -22,24 +22,29 @@ instance : Coe Nat Lambda := ⟨λ n => Lambda.var n⟩
 
 instance : OfNat Lambda n := ⟨Lambda.var n⟩
 
-def Lambda.shift (c i : Nat) : Lambda → Lambda
+namespace Lambda
+
+@[simp]
+def shift (c i : Nat) : Lambda → Lambda
   | var n =>
     if n < c then var n
     else var (n + i)
   | app e₁ e₂ => app (e₁.shift c i) (e₂.shift c i)
   | abs e => abs $ e.shift (c + 1) i
 
-def Lambda.unshift (c i : Nat) : Lambda → Lambda
+@[simp]
+def unshift (c i : Nat) : Lambda → Lambda
   | var n =>
     if n < c then var n
     else var (n - i)
   | app e₁ e₂ => app (e₁.unshift c i) (e₂.unshift c i)
   | abs e => abs $ e.unshift (c + 1) i
 
-notation:60 "↑"  c:61  i:62  t:63 => Lambda.shift c i t
-notation:60 "↓"  c:61  i:62  t:63 => Lambda.unshift c i t
+notation:70 "↑" => Lambda.shift
+notation:70 "↓" => Lambda.unshift
 
-def Lambda.subst (v : Lambda) (n : Nat) (e : Lambda) :=
+@[simp]
+def subst (v : Lambda) (n : Nat) (e : Lambda) :=
   match v with
   | var m =>
     if m = n then e
@@ -47,10 +52,20 @@ def Lambda.subst (v : Lambda) (n : Nat) (e : Lambda) :=
   | app v₁ v₂ => app (v₁.subst n e) (v₂.subst n e)
   | abs v₁ => abs $ v₁.subst (n + 1) (e.shift 0 1)
 
-notation:65 t:65 "[" k " ↦ " s:65 "]" => Lambda.subst t k s
+notation t " [" k " ↦ " s "]" => Lambda.subst t k s
+
+def beta (M N : Lambda) := (↓) 0 1 (M[0 ↦ (↑) 0 1 N])
+
+@[simp]
+def range : Lambda → Nat
+  | var n => n
+  | app e₁ e₂ => max (e₁.range) (e₂.range)
+  | abs e => e.range + 1
+
+end Lambda
 
 inductive Beta : Lambda → Lambda → Prop
-  | basis (M N : Lambda) : Beta ((λ M).app N) ((M.subst 0 (N.shift 0 1)).unshift 0 1)
+  | basis (M N : Lambda) : Beta ((λ M).app N) (Lambda.beta M N)
   | appr (M N L : Lambda) : Beta N M → Beta (N.app L) (M.app L)
   | appl (M N L : Lambda): Beta N M → Beta (L.app N) (L.app M)
   | abs (N M) : Beta N M → Beta (λ N) (λ M)
@@ -59,7 +74,7 @@ infixl:65 " →β " => Beta
 
 inductive BetaTR : Lambda → Lambda → Prop
   | refl (M) : BetaTR M M
-  | beta (M N) : Beta M N → BetaTR M N
+  | beta (M N) : M →β N → BetaTR M N
   | trans (M N L) : BetaTR M N → BetaTR N L → BetaTR M L
 
 infixl:65 " ⇒β " => BetaTR
