Lambda/Properties.lean
@@ -1,13 +1,13 @@
 import Lambda.Defs
 open Lambda
 
-theorem shift_var_le {c i n : Nat}  : c ≤ n → shift c i (var n) = var (n + i) := by
+theorem shift_var_le {c i n : Nat}  : c ≤ n → (↑) c i n = n + i := by
   intro h
   unfold shift
   have nnltc : ¬ (n < c) := Nat.not_lt.mpr h
   simp [nnltc]
 
-theorem shift_var_lt {c i n : Nat} : n < c → shift c i (var n) = var n := by
+theorem shift_var_lt {c i n : Nat} : n < c → (↑) c i n = n := by
   intro h; unfold shift; simp [h]
 
 theorem unshift_var_le {c i n : Nat} :
@@ -17,10 +17,10 @@ theorem unshift_var_le {c i n : Nat} :
   have nnltc : ¬ (n < c) := Nat.not_lt.mpr h
   simp [nnltc]
 
-theorem unshift_var_lt {c i n : Nat} : n < c → unshift c i (var n) = var n := by
+theorem unshift_var_lt {c i n : Nat} : n < c → (↓) c i n = var n := by
   intro h; unfold unshift; simp [h]
 
-theorem shift_zero {N : Lambda} : ∀ {c}, shift c 0 N = N := by
+theorem shift_zero {N : Lambda} : ∀ {c}, (↑) c 0 N = N := by
   induction N with
   | var n =>
     intro c
@@ -35,15 +35,15 @@ theorem shift_zero {N : Lambda} : ∀ {c}, shift c 0 N = N := by
     unfold shift <;> simp [ih]
 
 
-theorem shift_add {N : Lambda} :
-  ∀ {c i₁ i₂ : Nat}, shift c i₁ (shift c i₂ N) = shift c (i₁ + i₂) N := by
+theorem shift_add' (N : Lambda) :
+  ∀ {c i₁ i₂ : Nat}, (↑) c i₁ ((↑) c i₂ N) = (↑) c (i₁ + i₂) N := by
   induction N with
   | var n =>
     intro c i₁ i₂
     by_cases h : n < c
-    . simp [shift_var_lt h]
+    . simp [shift_var_lt h, h]
     . have clen : c ≤ n := Nat.le_of_not_lt h
-      simp_all [shift_var_le clen, shift_var_le <| Nat.le_add_right_of_le clen]
+      simp [h, shift_var_le <| Nat.le_add_right_of_le clen]
       ac_nf
   | app N₁ N₂ ih₁ ih₂ =>
     intro c i₁ i₂
@@ -55,3 +55,149 @@ theorem shift_add {N : Lambda} :
     rw [shift]
     unfold shift
     simp [ih]
+
+-- * ∀ (i j : Nat), i ≤ j → j ≤ i + m → ↑ j n (↑ i m N) = ↑ i (m + n) N
+theorem shift_add (n m : Nat) (N : Lambda)
+  : ∀ (i j : Nat), i ≤ j → j ≤ i + m → (N.shift i m).shift j n = N.shift i (m + n)
+  := by
+  induction N with
+  | var k =>
+    intro i j ilej jlem1
+    simp_all [Lambda.shift]
+    rcases Nat.lt_trichotomy k i with klei | rfl | kgti
+    -- * Case k < i
+    . simp [klei]
+      intro h
+      have : j < i := Nat.lt_of_le_of_lt h klei
+      have : j < j := Nat.lt_of_lt_of_le this ilej
+      have : ¬ j < j := Nat.lt_irrefl j
+      contradiction
+    -- * Case k = i
+    . simp [Nat.not_lt.mpr jlem1]; ac_nf
+    -- * Case k > i
+    . have : i + m < k + m := Nat.add_lt_add_right kgti m
+      have : j < k + m := Nat.lt_of_le_of_lt jlem1 this
+      have : ¬ k + m < j := Nat.not_lt_of_gt this
+      simp [Nat.not_lt_of_gt kgti, this]
+      ac_nf
+  | app e v ihe ihv =>
+    intro i j ilej jlemi
+    simp_all
+  | abs e ih =>
+    intro i j ilej jleim
+    simp_all
+    apply ih
+    exact Nat.add_le_add_right ilej 1
+    rw [Nat.add_assoc, Nat.add_comm 1 m, ← Nat.add_assoc]
+    exact Nat.add_le_add_right jleim 1
+
+-- (↑) 0 1 ((↑) i j L) =
+
+theorem shift_subst (N : Lambda) :
+  ∀ {n i j L}, i ≤ n → (↑) i j (N[n ↦ L]) = ((↑) i j N)[n + j ↦ (↑) i j L] := by
+  induction N with
+  | var m =>
+    intro n i j L ilen
+    simp
+    rcases Nat.lt_trichotomy m i with mlei | rfl | mgti
+    -- * Case m < i
+    . have nlen : m < n := Nat.lt_of_lt_of_le mlei ilen
+      have mlenj : m < n + j := Nat.lt_add_right j nlen
+      have mneqnj : m ≠ n + j := by exact Nat.ne_of_lt mlenj
+      simp [Nat.ne_of_lt nlen, mlei, mneqnj]
+    -- * Case m = j
+    . by_cases hmn : m = n
+      -- * Sub Case m = n
+      . simp [hmn]
+      -- * Sub Case m ≠ n
+      . simp [hmn]
+    -- * Case m > j
+    . simp [Nat.not_lt_of_gt mgti]
+      by_cases hmn : m = n
+      -- * Sub case m = n
+      . simp [hmn]
+      -- * Sub case m ≠ n
+      . simp [hmn]
+        intro mlei
+        have mlem : m < m := Nat.lt_trans mlei mgti
+        have : ¬ m < m := Nat.lt_irrefl m
+        contradiction
+    | app N₁ N₂ ih1 ih2 =>
+      intro n i j L ilen
+      simp <;> repeat (first | constructor | exact ih1 ilen | exact ih2 ilen )
+    | abs N ih =>
+      intro n i j L ilen
+      have : i + 1 ≤ n + 1 := Nat.add_le_add_right ilen 1
+      simp
+      sorry
+
+theorem subst_gt_range {M} : ∀ {N n}, n > range M → M[n ↦ N] = M := by
+  induction M with
+  | var m =>
+    intro N n h
+    unfold range at h
+    simp [Nat.ne_of_lt h]
+  | app M₁ M₂ ih1 ih2 =>
+    intro N n h
+    unfold range at h
+    have ⟨ngt1, ngt2⟩ := Nat.max_lt.mp h
+    simp [ih1 ngt1, ih2 ngt2]
+  | abs M ih =>
+    intro N n h
+    unfold range at h
+    have ngtrm1 : n + 1 > range M := Nat.lt_of_succ_lt <| Nat.lt_add_right 1 h
+    simp  [ih ngtrm1]
+
+theorem gt_range_gt_shift {N : Lambda} :
+  ∀ {n i j}, n > range N → n + j > range ((↑) i j N) := by
+  induction N with
+  | var m =>
+    intro n i j h
+    unfold range at h
+    simp [shift]
+    by_cases mi : m < i
+    -- * case m < i
+    . simp [mi, Nat.lt_add_right j h]
+    -- * Case ¬ m < i
+    . simp [mi, h]
+  | app N₁ N₂ ih1 ih2 =>
+    intro n i j h
+    unfold range at h
+    have ⟨ngt1, ngt2⟩ := Nat.max_lt.mp h
+    unfold shift range
+    apply Nat.max_lt.mpr
+    constructor <;> repeat (first | apply ih1 | apply ih2 | assumption)
+  | abs N ih =>
+    intro n i j h
+    unfold range at h
+    have : n - 1 > range N := Nat.lt_sub_of_add_lt h
+    have := @ih (n - 1) (i + 1) j this
+    have : n + j > ((↑) (i + 1) j N).range + 1 := by sorry
+    simp [shift, range]
+    assumption
+
+theorem sustitution {M N L: Lambda} :
+  ∀ {n m N L}, n ≠ m → n > range L → M[n ↦ N][m ↦ L] = M[m ↦ L][n ↦ N[m ↦ L]] := by
+  induction M with
+  | var k =>
+    intro n m N L mneqn ngtrl
+    by_cases h : k = n
+    -- * Case k = m
+    . simp [h, mneqn]
+    -- * case k ≠ m
+    . simp [h]
+      by_cases h' : k = m
+      -- * case k = m
+      . simp [h', subst_gt_range ngtrl]
+      -- * Case k ≠ m
+      . simp [h', h]
+  | app M₁ M₂ ih1 ih2 =>
+    intro n m N L nneqm ngtrl
+    simp [ih1 nneqm ngtrl, ih2 nneqm ngtrl]
+  | abs M ih =>
+    intro n m N L nneqm ngtrl
+    have h1 : n + 1 ≠ m + 1 := by sorry
+    have : n + 1 > range ((↑) 0 1 L) := gt_range_gt_shift ngtrl
+    have := @ih (n + 1) (m + 1) ((↑) 0 1 N) ((↑) 0 1 L) h1 this
+    simp
+    sorry
